lib/fst/Lib.Buffer.fst
@@ -144,6 +144,11 @@ let salloc1 #a #res h len x footprint spec spec_inv impl =
   r
 
 inline_for_extraction noextract
+let salloc1_trivial #a #res h len x footprint spec impl =
+  let trivial (#res:Type) (h1 h2 h3:mem) (r:res) = () in
+  salloc1 h len x footprint spec trivial impl
+
+inline_for_extraction noextract
 val loopi_blocks_f:
     #a:Type0
   -> #b:Type0
